HashMap lemmas

src/Std/Data/HashMap/Basic.lean
@@ -198,6 +198,10 @@ instance [BEq α] [Hashable α] : GetElem? (HashMap α β) α β (fun m a => a �
     HashMap α Unit :=
   ⟨DHashMap.Const.unitOfList l⟩
 
+@[inline, inherit_doc DHashMap.Const.ofList] def ofArray [BEq α] [Hashable α] (a : Array (α × β)) :
+    HashMap α β :=
+  ⟨DHashMap.Const.ofArray a⟩
+
 @[inline, inherit_doc DHashMap.Const.toList] def toList (m : HashMap α β) :
     List (α × β) :=
   DHashMap.Const.toList m.inner
